pulse/share/pulse/examples/bug-reports/PulseTest.UseLang.fst
@@ -1,30 +1,42 @@
 module PulseTest.UseLang
 #lang-pulse
-open FStar.Mul
 open Pulse.Lib.Pervasives
+
+fn double (x:ref int)
+requires pts_to x 'v
+ensures pts_to x ('v + 'v)
+{
+  open FStar.Mul; //dependence scanning works inside Pulse
+  let v = !x;
+  x := 2 * v;
+}
+
 let x = 0
+
 let y = 1
-let z = x + y 
+
+let z = x + y
+
 let w = z
+
 let t = 0
 
 fn return_z ()
 requires emp
 returns r:int
 ensures pure (r == z)
-{  //add some comments; it caches fine
-    z
+{
+  z
 }
 
-
 let some = 1
-let foobar = 17 
 
+let foobar = 17
 
 fn return_2z ()
 requires emp
 returns r:int
-ensures pure (r == 2 * z)
+ensures pure (FStar.Mul.(r == 2 * z)) //dep scanning inside Pulse
 {
   let v = return_z ();
   (v + x + y)
